**[[Cuaderno de trabajo.pdf|Archivo PDF]]**

## Evaluaciones en aula

### Evaluaci√≥n en aula 1

#### Modelo 1

##### Pregunta 1

**a)**

$$
\begin{align}
\vec{A} + \vec{B} &= -3\hat{i} - 4\hat{j} + \hat{k} - 5\hat{i} + 6\hat{j} + 6\hat{k} \\
\vec{A} + \vec{B} &= -8\hat{i} + 2\hat{j} + 7\hat{k}
\end{align}
$$

$$
\begin{align}
\vec{u} &= \frac{\vec{A} + \vec{B}}{\lVert \vec{A} + \vec{B} \rVert} \\
&= \frac{-8\hat{i} + 2\hat{j} + 7\hat{k}}{\sqrt{(-8)^{2} + 2^{2} + 7^{2}}} = \frac{-8\hat{i} + 2\hat{j} + 7\hat{k}}{\sqrt{117}} \\
\vec{u} &= \left< -\frac{8}{\sqrt{117}}, \frac{2}{\sqrt{117}}, \frac{7}{\sqrt{117}} \right> 
\end{align}
$$

**b)**

$$
\begin{align}
\lVert \vec{A} - \vec{C} \rVert &= \sqrt{(-3 -4)^{2} + (-4 - 3)^{2} + (1 + 7)^{2}} \\
&= \sqrt{49 + 49 + 64} \\
&= \sqrt{162}
\end{align}
$$

**c)**

$$
\begin{align}
\theta &= \arccos\left( \frac{\vec{B} \cdot \vec{C}}{\lVert \vec{B} \rVert \lVert \vec{C} \rVert } \right) \\
&= \arccos\left( \frac{(-5)(4)+(6)(3) + (6)(-7)}{\sqrt{(-5)^{2} + 6^{2} + 6^{2}} \cdot \sqrt{4^{2} + 3^{2} + (-7)^{2}}}\right) \\
&= \arccos \left( -\frac{44}{84.72} \right) \\
&= \arccos \left( -\frac{44}{84.72} \right)  \\
\theta &= 121.29\degree
\end{align}
$$

**d)**

$$
\vec{B} + \vec{C} = -\hat{\mathbf{i}} + 9\hat{\mathbf{j}} - \hat{\mathbf{k}}
.$$

Luego,

$$
\begin{align}
\operatorname{comp}_{\vec{B}+\vec{C}}(\vec{A}) &= \frac{\vec{A} \cdot (\vec{B + C})}{\lVert \vec{B} + \vec{C} \rVert } \\
&= \frac{(-3\hat{\mathbf{i}} -4\hat{\mathbf{j}} + \hat{\mathbf{k}}) \cdot (-\hat{\mathbf{i}} + 9\hat{\mathbf{j}} - \hat{\mathbf{k}})}{\sqrt{1^{2} + 9^{2} + 1^{2}}} \\
&= \frac{(-3)(-1) + (-4)(9) + (1)(-1)}{\sqrt{83}} \\
\operatorname{comp}_{\vec{B}+\vec{C}}(\vec{A})& = -\frac{34}{\sqrt{83}} \\
\end{align}
$$

y por lo tanto

$$
\begin{align}
\operatorname{proy}_{\vec{B}+\vec{C}}(\vec{A}) &= -\frac{34}{\sqrt{83}} \cdot \frac{\vec{B}+\vec{C}}{\lVert \vec{B} + \vec{C} \rVert } \\
&= -\frac{34}{\sqrt{83}} \cdot \frac{-\hat{\mathbf{i}} + 9\hat{\mathbf{j}} - \hat{\mathbf{k}}}{\sqrt{83}} \\
&= \frac{34}{83}\hat{\mathbf{i}} - \frac{306}{83}\hat{\mathbf{j}} + \frac{34}{83}\hat{\mathbf{k}}
\end{align}
$$
